\documentclass{article}
\usepackage{CJKutf8}
\usepackage{amsmath}
\usepackage{amssymb}
\usepackage{amsfonts}
\usepackage{amsthm}
\usepackage{titlesec}
\usepackage{titletoc}
\usepackage{xCJKnumb}
\usepackage{tikz}
\usepackage{mathrsfs}
\usepackage{indentfirst}
\usepackage{enumitem}
\newtheorem{Def}{定义}
\newtheorem{Thm}{定理}
\newtheorem{Exercise}{练习}

\newtheorem*{Example}{例}
\setlist[enumerate,1]{label=(\arabic*)}

\begin{document}
\begin{CJK*}{UTF8}{gbsn}
  \title{第三讲 联结词的扩充与规约}
  \author{陈建文}
  \maketitle
  % \tableofcontents

  课后作业题：
  \begin{Exercise}
    用$\{\lnot,\to\}$等价表示下列公式：
    \[(p\lor(p\land q))\leftrightarrow p\]
  \end{Exercise}

  \begin{proof}[解]
    \begin{align*}
      &(p\lor(p\land q))\leftrightarrow p\\
      \Leftrightarrow&((p\lor(p\land q))\to p)\land (p\to (p\lor(p\land q)))\\
      \Leftrightarrow&(\lnot (p\lor(p\land q))\lor p)\land (\lnot p \lor (p\lor(p\land q)))\\
      \Leftrightarrow&(\lnot (p\lor(p\land q))\lor p\\
      \Leftrightarrow&(\lnot p \land \lnot (p\land q))\lor p\\
      \Leftrightarrow&(\lnot p\land \lnot p)\lor (\lnot p\land \lnot q)\lor p\\
      \Leftrightarrow&\lnot p\lor (\lnot p\land \lnot q)\lor p\\
      \Leftrightarrow&\lnot p \lor p\\
      \Leftrightarrow&p \to p\\
    \end{align*}
    
  \end{proof}
  \begin{Exercise}
    用$\{\uparrow, \downarrow \}$分别等价表示下列公式：
    \begin{enumerate}
      \item $\lnot p\lor q$
      \item $p\land \lnot q$
      \item $\lnot p \lor \lnot q$
      \item $p\leftrightarrow q$
    \end{enumerate}
    
  \end{Exercise}

  \begin{proof}[解]
    \begin{align*}
      (1)&\lnot p\lor q\Leftrightarrow(p\downarrow p)\lor q
      \Leftrightarrow\lnot \lnot ((p\downarrow p)\lor q)
      \Leftrightarrow\lnot ((p\downarrow p)\downarrow q)\\
      &\Leftrightarrow ((p\downarrow p)\downarrow q)\downarrow ((p\downarrow p)\downarrow q)\\
      &\lnot p\lor q
      \Leftrightarrow\lnot\lnot (\lnot p \lor q)
      \Leftrightarrow\lnot (p \land \lnot q)
      \Leftrightarrow p\uparrow \lnot q
      \Leftrightarrow p\uparrow(q\uparrow q)\\ 
      (2)&p\land \lnot q
      \Leftrightarrow\lnot\lnot (p\land \lnot q)
      \Leftrightarrow\lnot (\lnot p \lor q)
      \Leftrightarrow(\lnot q)\downarrow q
      \Leftrightarrow(p\downarrow p)\downarrow q\\
      &p\land \lnot q
      \Leftrightarrow  \lnot \lnot (p\land \lnot q)
      \Leftrightarrow  \lnot (p\uparrow \lnot q)
      \Leftrightarrow(p\uparrow \lnot q)\uparrow (p\uparrow \lnot q)\\
      &\Leftrightarrow(p\uparrow (q\uparrow q))\uparrow (p\uparrow (q\uparrow q))\\
      (3)&\lnot p \lor \lnot q
      \Leftrightarrow \lnot\lnot (\lnot p \lor \lnot q)
      \Leftrightarrow \lnot (p \land q)
      \Leftrightarrow p\uparrow q\\
      &\lnot p \lor \lnot q
      \Leftrightarrow \lnot\lnot (\lnot p \lor \lnot q)
      \Leftrightarrow \lnot (\lnot p\downarrow \lnot q)
      \Leftrightarrow (\lnot p\downarrow \lnot q)\downarrow(\lnot p\downarrow \lnot q)\\
      &\Leftrightarrow (( p\downarrow p)\downarrow ( q\downarrow q))\downarrow(( p\downarrow p)\downarrow ( q\downarrow q))\\
      (4)&p\leftrightarrow q\Leftrightarrow (p\to q)\land (q\to p)\Leftrightarrow (\lnot p \lor q) \land (\lnot q\lor p) \Leftrightarrow \lnot \lnot (\lnot p \lor q) \land \lnot\lnot(\lnot q\lor p)\\
      &\Leftrightarrow\lnot (p\land \lnot q)\land \lnot (q\land \lnot p)\Leftrightarrow (p\uparrow \lnot q)\land (q\uparrow \lnot p)\Leftrightarrow \lnot\lnot ((p\uparrow \lnot q)\land (q\uparrow \lnot p))\\
      &\Leftrightarrow  \lnot((p\uparrow \lnot q)\uparrow (q\uparrow \lnot p))\Leftrightarrow\lnot((p\uparrow  (q\uparrow q))\uparrow (q\uparrow (p\uparrow p)))\\
      &\Leftrightarrow((p\uparrow  (q\uparrow q))\uparrow (q\uparrow (p\uparrow p)))\uparrow ((p\uparrow  (q\uparrow q))\uparrow (q\uparrow (p\uparrow p)))\\
      &p\leftrightarrow q\Leftrightarrow (p\to q)\land (q\to p)\Leftrightarrow (\lnot p \lor q) \land (\lnot q\lor p) \Leftrightarrow\lnot \lnot ((\lnot p \lor q) \land (\lnot q\lor p))\\
      &\Leftrightarrow \lnot (\lnot (\lnot p \lor q) \lor \lnot (\lnot q\lor p)) \Leftrightarrow \lnot ((\lnot p \downarrow q) \lor (\lnot q\downarrow p)) \Leftrightarrow (\lnot p \downarrow q) \downarrow (\lnot q\downarrow p) \\
      &\Leftrightarrow( (p\downarrow p) \downarrow q) \downarrow ((q\downarrow q)\downarrow p)
    \end{align*}
  \end{proof}
\end{CJK*}
\end{document}





%%% Local Variables:
%%% mode: latex
%%% TeX-master: t
%%% End: